ocaml/lib/extracted/Xp.mli
@@ -1,3 +1,4 @@
+open Datatypes
 open Equalities
 open Features
 open Utils
@@ -7,6 +8,77 @@ module type FeatureSig =
   val n : int
 
   val fs : featureSig
+ end
+
+module FeatureSigDefs :
+ functor (F:FeatureSig) ->
+ functor (S:sig
+  module E :
+   sig
+    type t = fin
+
+    val compare : t -> t -> comparison
+
+    val eq_dec : t -> t -> bool
+   end
+
+  type elt = E.t
+
+  type t
+
+  val empty : t
+
+  val is_empty : t -> bool
+
+  val mem : elt -> t -> bool
+
+  val add : elt -> t -> t
+
+  val singleton : elt -> t
+
+  val remove : elt -> t -> t
+
+  val union : t -> t -> t
+
+  val inter : t -> t -> t
+
+  val diff : t -> t -> t
+
+  val equal : t -> t -> bool
+
+  val subset : t -> t -> bool
+
+  val fold : (elt -> 'a1 -> 'a1) -> t -> 'a1 -> 'a1
+
+  val for_all : (elt -> bool) -> t -> bool
+
+  val exists_ : (elt -> bool) -> t -> bool
+
+  val filter : (elt -> bool) -> t -> t
+
+  val partition : (elt -> bool) -> t -> t * t
+
+  val cardinal : t -> int
+
+  val elements : t -> elt list
+
+  val choose : t -> elt option
+
+  val eq_dec : t -> t -> bool
+
+  val compare : t -> t -> comparison
+
+  val min_elt : t -> elt option
+
+  val max_elt : t -> elt option
+
+  val all : t
+
+  val compl : t -> t
+
+  val shrink : (t -> bool) -> t -> t
+ end) ->
+ sig
  end
 
 module type Output =
